Deploying to gh-pages from @ xubaiw/reservoir-index@2f87a4a531528c3b3eaba917bfed674c50acc477 🚀

git/jrr6/lean-tables/Table/API.lean
@@ -428,6 +428,612 @@ by intros xs k
        apply Nat.succ_le_succ
        exact ih
 
+theorem findMatches_lengths_sum {κ ν} [inst : DecidableEq κ] :
+  ∀ (xs : List (κ × ν)) (k : κ),
+  (findMatches xs k).1.length + (findMatches xs k).2.length = xs.length :=
+by intros xs k
+   induction xs with
+   | nil => rfl
+   | cons x xs ih =>
+     simp only [findMatches]
+     cases inst x.1 k with
+     | isFalse hfalse =>
+       simp only [hfalse, ite_false, List.length]
+       rw [←Nat.add_assoc]
+       apply congrArg (·+1) ih
+     | isTrue htrue =>
+       simp only [htrue, ite_true, List.length]
+       rw [Nat.add_assoc, Nat.add_comm 1, ←Nat.add_assoc]
+       apply congrArg (·+1) ih
+
+theorem findMatches_snd_keys_neq_k_map [DecidableEq κ] (xs : List (κ × ν)) :
+  ∀ e, e ∈ (List.map Prod.fst (findMatches xs k).snd) → e ≠ k :=
+by intros e hsnd
+   induction xs with
+   | nil => cases hsnd
+   | cons x xs ih =>
+     cases Decidable.em (x.1 = k) with
+     | inl heq =>
+       apply ih
+       simp only [findMatches, heq, ite_true] at hsnd
+       exact hsnd
+     | inr hneq =>
+       simp only [findMatches, hneq, ite_false] at hsnd
+       cases hsnd with
+       | head => exact hneq
+       | tail _ hin => exact ih hin
+
+theorem List.fst_mem_of_pair_mem : ∀ (x : α) (y : β) (ps : List (α × β)),
+  (x, y) ∈ ps → x ∈ (map Prod.fst ps)
+| x, y, [], hxy => by contradiction
+| x, y, _ :: ps, List.Mem.head _ _ => List.Mem.head _ _
+| x, y, _ :: ps, List.Mem.tail a ha => Mem.tail _ $ fst_mem_of_pair_mem x y ps ha
+
+theorem findMatches_snd_keys_neq_k [DecidableEq κ] (xs : List (κ × ν)) :
+  ∀ e, e ∈ (findMatches xs k).snd → e.fst ≠ k := λ e he =>
+findMatches_snd_keys_neq_k_map xs e.fst
+  (List.fst_mem_of_pair_mem e.1 e.2 (findMatches xs k).snd he)
+
+theorem List.reverse_singleton (x : α) : reverse [x] = [x] := rfl
+theorem List.singleton_append (x : α) (xs : List α) : [x] ++ xs = x :: xs := rfl
+
+-- TODO: should we use `List.eraseDups` instead? (Uses BEq instead of DEq.)
+def List.uniqueAux {α} [DecidableEq α] : List α → List α → List α
+| [], acc => acc.reverse
+| x :: xs, acc => if x ∈ acc then uniqueAux xs acc else uniqueAux xs (x :: acc)
+
+def List.unique {α} [DecidableEq α] (xs : List α) := uniqueAux xs []
+
+theorem List.all_pred {p : α → Prop} [DecidablePred p] {xs : List α} :
+  xs.all (λ x => decide (p x)) ↔ ∀ x, x ∈ xs → p x := by
+  simp only [all]
+  apply Iff.intro
+  . intros hforward x hx
+    induction hx with
+    | head a as =>
+      simp [foldr] at hforward
+      apply And.left hforward
+    | tail a h ih =>
+      apply ih
+      simp [foldr] at hforward
+      apply And.right hforward
+  . intros hbackward
+    induction xs with
+    | nil => simp [foldr]
+    | cons x xs ih =>
+      simp [foldr]
+      apply And.intro
+      . apply hbackward x (List.Mem.head _ _)
+      . apply ih
+        intro x' hx'
+        apply hbackward _ $ List.Mem.tail _ hx'
+
+@[instance] def List.forAllDecidable (xs : List α) (p : α → Prop) [DecidablePred p] : Decidable (∀x, x ∈ xs → p x) :=
+if h : xs.all (λ x => decide (p x))
+then Decidable.isTrue (List.all_pred.mp h)
+else Decidable.isFalse (h ∘ List.all_pred.mpr)
+
+-- TODO: try just making this the function since both of them are n²
+def List.unique' {α} [DecidableEq α] : List α → List α
+| [] => []
+| x :: xs =>
+  let ys := unique' xs
+  if ∀ y, y ∈ ys → x ≠ y then x :: ys else ys
+
+-- TODO: If we could just state some sort of meaningful spec for `uniqueAux`,
+-- everything would be golden...
+theorem List.uniqueAux_eq_acc_append_xs {α} [DecidableEq α] (xs acc : List α) :
+  uniqueAux xs acc = (reverse acc) ++ unique xs :=
+by induction xs with
+   | nil => simp [uniqueAux, unique]
+   | cons x xs ih =>
+     simp only [uniqueAux, unique, List.not_mem_nil, ite_false]
+     cases Decidable.em (x ∈ acc) with
+     | inl hin =>
+       simp only [hin, ite_true, ih]
+
+theorem List.unique_eq_uniqueSpec {α} [DecidableEq α] :
+  ∀ (xs : List α), unique xs = unique' xs
+| [] => rfl
+| x :: xs => by
+  simp only [unique, unique', uniqueAux, not_mem_nil, ite_false]
+
+-- theorem List.length_uniqueAux {α} [DecidableEq α] (xs : List α) :
+--   ∀ (acc : List α),
+--   length (uniqueAux xs acc) = length (unique xs) + length acc :=
+-- by induction xs with
+--    | nil => 
+--      intros
+--      simp only [unique, uniqueAux, length_reverse, length, Nat.zero_add]
+--    | cons x xs ih =>
+--      intros acc h
+--      simp only [uniqueAux, unique, List.not_mem_nil, ite_false]
+--      split
+--      . simp only [length, ih]
+--        rw [Nat.add_assoc]
+--        apply congrArg
+--        rw [Nat.zero_add]
+--        conv => lhs; rw [←Nat.zero_add (length acc)]
+--        apply congrArg (·+ length acc)
+--        admit
+--      . simp only [length, ih]
+--        rw [Nat.add_assoc]
+--        apply congrArg
+--        apply Nat.add_comm
+
+theorem List.reverseAux_append :
+  reverseAux xs acc = (reverse xs) ++ acc :=
+by induction xs generalizing acc with
+   | nil => simp [reverseAux]
+   | cons x xs ih =>
+     simp only [reverse, reverseAux]
+     -- TODO: something's up here -- there shouldn't be two IHs
+     -- Deal with after sorting out `unique`
+     conv => rhs; rw [ih]
+     rw [append_assoc, singleton_append]
+     exact ih
+
+theorem List.uniqueAux_weak_existential {α} [DecidableEq α] (xs : List α)
+  (acc : List α) : ∃ ys, uniqueAux xs acc = reverse acc ++ ys := by
+  induction xs generalizing acc with
+  | nil => apply Exists.intro []; simp [uniqueAux]
+  | cons x xs ih =>
+    simp only [uniqueAux]
+    cases Decidable.em (x ∈ acc) with
+    | inl hin => simp only [hin, ite_true]; exact ih _
+    | inr hout =>
+      simp only [hout, ite_false]
+      have ih_inst := ih (x :: acc)
+      simp only [reverse, reverseAux] at ih_inst
+      rw [reverseAux_append] at ih_inst
+      cases ih_inst with | intro ys hys =>
+      apply Exists.intro (x :: ys)
+      conv => rhs; rw [←singleton_append, ←append_assoc]
+      exact hys
+
+theorem List.mem_singleton_iff (x y : α) : x ∈ [y] ↔ x = y := by
+  apply Iff.intro
+  . intros hin
+    cases hin
+    . rfl
+    . contradiction
+  . intros heq
+    rw [heq]
+    apply Mem.head
+
+theorem List.mem_cons_iff_mem_singleton_or_tail (y : α) (ys : List α) (x : α) :
+  x ∈ y :: ys ↔ x ∈ [y] ∨ x ∈ ys := by
+  apply Iff.intro
+  . intro hf
+    cases hf with
+    | head => apply Or.intro_left _ (Mem.head _ _)
+    | tail _ h => apply Or.intro_right _ h
+  . intro hb
+    cases hb with
+    | inl h => rw [(mem_singleton_iff x y).mp h]; apply Mem.head
+    | inr h => apply Mem.tail _ h
+
+-- TODO: could maybe fix things by using `&&` here instead of `∧`
+theorem List.filter_filter (p₁ p₂ : α → Bool) (xs : List α) :
+  filter p₁ (filter p₂ xs) = filter (λ x => p₂ x ∧ p₁ x) xs := by
+  -- filter p₁ (filter p₂ xs) = filter (λ x => p₂ x ∧ p₁ x) xs := by
+  rw [filter_eq_filterSpec, filter_eq_filterSpec, filter_eq_filterSpec]
+  induction xs with
+  | nil => simp [filterSpec]
+  | cons x xs ih =>
+    cases h₂ : p₂ x with
+    | false =>
+      simp only [filterSpec, h₂, ite_false]
+      exact ih
+    | true =>
+      simp only [filterSpec, h₂, ite_true]
+      cases h₁ : p₁ x with
+      | false =>
+        simp only [filterSpec, h₁, h₂, ite_false]
+        exact ih
+      | true =>
+        simp only [filterSpec, h₁, h₂, ite_true]
+        exact congrArg _ ih
+
+-- TODO: figure out where De Morgan's laws are hiding in the library...
+-- (There's `Decidable.not_and_iff_or_not`, but why shoul we require
+-- decidability?)
+theorem not_or_distrib : ¬ (a ∨ b) ↔ ¬a ∧ ¬b :=
+Iff.intro
+(λ h => And.intro (λ ha => h (Or.intro_left _ ha))
+                  (λ hb => h (Or.intro_right _ hb)))
+(λ h => λ hneg =>
+  match hneg with
+  | Or.inl ha => h.left ha
+  | Or.inr hb => h.right hb)
+
+-- Again, this must be in the library somewhere...
+theorem And.comm : p ∧ q ↔ q ∧ p :=
+  Iff.intro (λ h => And.intro h.right h.left) (λ h => And.intro h.right h.left)
+
+theorem not_iff_not_of_iff : (p ↔ q) → (¬ p ↔ ¬ q) := λ hpq =>
+  Iff.intro (λ hnp hq => hnp $ hpq.mpr hq) (λ hnq hp => hnq $ hpq.mp hp)
+
+-- set_option pp.explicit true
+
+theorem iff_true_intro (h : a) : a ↔ true :=
+Iff.intro
+  (λ hl => rfl)
+  (λ hr => h)
+theorem eq_true_intro {a : Prop} (h : a) : a = true :=
+propext (iff_true_intro h)
+
+theorem decide_type_eq (p q : Prop) [ip : Decidable p] [iq : Decidable q] :
+  p = q → decide p = decide q := λ h =>
+  by cases h
+     apply congr
+     . simp
+     . apply eq_of_heq
+       apply Subsingleton.helim
+       rfl
+
+theorem List.uniqueAux_acc_append_filter {α} [DecidableEq α] :
+  ∀ (xs acc : List α),
+  uniqueAux xs acc = reverse acc ++ unique (xs.filter (· ∉ acc))
+| [], acc => by simp [uniqueAux, reverse, reverseAux, unique]
+| x :: xs, acc =>
+  have hterm : length (filter (λ a => !decide (a ∈ acc)) xs)
+                < Nat.succ (length xs) :=
+    Nat.lt_of_le_of_lt (m := length xs) (filter_length _ _) (Nat.lt.base _)
+  have ih₁ := uniqueAux_acc_append_filter xs acc
+  have ih₂ := uniqueAux_acc_append_filter xs (x :: acc)
+  have ih₃ :=
+    uniqueAux_acc_append_filter (filter (λ a => decide ¬a ∈ acc) xs) [x]
+  by
+    simp only [uniqueAux, filter, filterAux]
+    cases Decidable.em (x ∈ acc) with
+    | inl hin =>
+      simp only [hin, ite_true]
+      -- TODO: this shouldn't be necessary
+      have : decide False = false := rfl
+      rw [this]
+      simp only
+      rw [ih₁]
+      simp only [filter]
+    | inr hout =>
+      -- Case x is not already in the accumulator
+      simp only [hout, ite_false]
+      have : decide True = true := rfl
+      rw [this]
+      simp only [filterAux_spec, reverse_singleton, singleton_append, unique,
+                 uniqueAux, List.not_mem_nil, ite_false]
+      rw [ih₂]
+      simp only [reverse_cons, append_assoc, singleton_append]
+      apply congrArg
+      simp only [unique]
+      rw [ih₃]
+      rw [reverse_singleton, singleton_append, filter_filter]
+      have : (λ x_1 => decide (
+              (decide ¬x_1 ∈ acc) = true ∧ (decide ¬x_1 ∈ [x]) = true)
+             ) = (λ x_1 => decide (¬x_1 ∈ acc ∧ ¬x_1 ∈ [x])) :=
+        by simp
+      rw [this, ←unique]
+      apply congrArg
+      apply congrArg
+      have h_mem_iff := mem_cons_iff_mem_singleton_or_tail x acc
+      have h_mem_iff_neg := (λ x => not_iff_not_of_iff $ h_mem_iff x)
+      apply congr _ rfl
+      apply congr rfl
+      apply funext
+      intros a
+      apply decide_type_eq
+      rw [h_mem_iff_neg, not_or_distrib, And.comm]
+termination_by uniqueAux_acc_append_filter xs ac => xs.length
+
+theorem List.uniqueAux_acc_append {α} [DecidableEq α] (xs : List α)
+  (acc : List α) (h : ∀ x, x ∈ xs → ¬ (x ∈ acc)) :
+  uniqueAux xs acc = reverse acc ++ unique xs := by
+  have : filter (fun a => decide ¬a ∈ acc) xs = xs := by
+    induction xs with
+    | nil => simp [filter, filterAux]
+    | cons x xs ih =>
+      simp only [filter, filterAux]
+      have : decide (¬x ∈ acc) = true := by simp [h x (Mem.head _ _)]
+      rw [this]
+      simp only
+      rw [filterAux_spec, ih, reverse_singleton, singleton_append]
+      . intros x hx
+        apply h x (Mem.tail _ hx)
+  rw [uniqueAux_acc_append_filter]
+  cases xs with
+  | nil => apply congrArg; simp [filter, filterAux]
+  | cons x xs =>
+    apply congrArg
+    rw [this]
+
+theorem List.length_uniqueAux {α} [DecidableEq α]
+  (xs : List α) (acc : List α) (h : ∀ x, x ∈ xs → ¬ (x ∈ acc)) :
+  length (uniqueAux xs acc) = length (unique xs) + length acc := by
+  rw [uniqueAux_acc_append _ _ h, length_append, length_reverse, Nat.add_comm]
+
+theorem findMatches_fst_eq_filter_k_map_snd {κ ν} [inst : DecidableEq κ] :
+  ∀ (xs : List (κ × ν)) (k : κ),
+    (findMatches xs k).1 = (xs.filter (λ x => x.1 = k)).map Prod.snd :=
+by intros xs k
+   simp only [List.filter]
+   induction xs with
+   | nil => rfl
+   | cons x xs ih =>
+     simp only [findMatches]
+     cases inst x.1 k with
+     | isFalse hfalse =>
+       simp only [hfalse, ite_false, List.filterAux, ih]
+       exact rfl
+     | isTrue htrue =>
+       simp only [htrue, ite_true, List.filterAux, ih]
+       -- TODO: why won't Lean reduce `match decide True with...` to the
+       -- `true` arm automatically? This workaround works but is ugly.
+       have h :
+        (x.2 :: List.map Prod.snd (List.filterAux
+            (λ x => decide (x.fst = k)) xs []) =
+          List.map Prod.snd
+            (match decide True with
+            | true => List.filterAux (fun x => decide (x.fst = k)) xs [x]
+            | false => List.filterAux (fun x => decide (x.fst = k)) xs []))
+        = (x.2 :: List.map Prod.snd (List.filterAux
+            (λ x => decide (x.fst = k)) xs []) =
+          List.map Prod.snd (List.filterAux
+            (fun x => decide (x.fst = k)) xs [x])) := rfl
+       simp only at h
+       apply cast (Eq.symm h)
+       have h_filterAux := List.filterAux_acc_eq_rev_append
+                            (λ x => decide (x.fst = k)) xs [x] []
+       rw [List.nil_append, List.reverse_singleton, List.singleton_append]
+        at h_filterAux
+       rw [h_filterAux]
+       simp only [List.map]
+
+def List.groupByKey {κ} [DecidableEq κ] {ν} : List (κ × ν) → List (κ × List ν)
+| [] => []
+| (k, v) :: kvs =>
+  have h_help : (findMatches kvs k).2.length < kvs.length.succ :=
+    Nat.lt_of_succ_le $ Nat.succ_le_succ $ findMatches_snd_length kvs k
+  
+  let fms := findMatches kvs k
+  (k, v :: fms.1) :: groupByKey fms.2
+termination_by groupByKey xs => xs.length
+decreasing_by assumption
+
+theorem List.groupByKey_findMatches_snd_length_cons [DecidableEq κ] 
+  (k : κ) (v : ν) (xs : List (κ × ν)) :
+  1 + length (groupByKey (findMatches ((k, v) :: xs) k).snd) = (groupByKey ((k, v) :: xs)).length :=
+calc
+  1 + length (groupByKey (findMatches ((k, v) :: xs) k).2)
+  = 1 + length (groupByKey (findMatches xs k).2) := by simp only [findMatches, length, ite_true]
+  _ = length (groupByKey (findMatches xs k).2) + 1 := Nat.add_comm _ _
+  _ = length ((k, v :: (findMatches xs k).1) :: groupByKey (findMatches xs k).2) := rfl
+  _ = length (groupByKey ((k, v) :: xs)) := rfl
+
+-- Or.intro_right _ $ Eq.symm $ calc
+--   length (groupByKey ((k, v) :: xs))
+--   = length ((k, v :: (findMatches xs k).1) :: groupByKey (findMatches xs k).2) := rfl
+--   _ = length (groupByKey (findMatches xs k).2) + 1 := rfl
+--   _ = 1 + length (groupByKey (findMatches xs k).2) := Nat.add_comm _ _
+--   _ = 1 + length (groupByKey (findMatches ((k, v) :: xs) k).2) := by simp [findMatches]
+
+
+  -- have ih := groupByKey_findMatches_snd_length (findMatches xs k).snd
+  -- Or.intro_right _ ( by
+  --   simp only [findMatches]
+  --   cases x with | mk curK curV =>
+  --   cases Decidable.em (curK = k) with
+  --   | inl heq =>
+  --      simp only [heq, ite_true, groupByKey]
+  --      conv => rhs; simp only [length]
+  --      apply Nat.add_comm
+  --   | inr hneq =>
+  --      simp [hneq, ite_false, groupByKey] -- TODO: strict simp set
+       
+  -- )
+-- :=
+-- by intros xs
+--    induction xs with
+--    | nil => apply Or.intro_left; rfl
+--    | cons x xs ih =>
+--      cases x with | mk curK curV =>
+--      simp only [findMatches]
+--      cases Decidable.em (curK = k) with
+--      | inl heq =>
+--        simp only [heq, ite_true, groupByKey]
+--        conv => rhs; simp only [length]
+--        apply Or.intro_right
+--        apply Nat.add_comm
+--      | inr hneq =>
+--        simp only [hneq, ite_false, groupByKey]
+--        conv => rhs; simp only [length]
+--        conv =>
+--         lhs
+--         simp only [length]
+--         rw [ih]
+
+theorem List.length_uniqueAux_findMatches {κ ν} [DecidableEq κ] (xs : List (κ × ν)) (k : κ) :
+  ∀ (acc : List κ) (hk : k ∈ acc),
+  (uniqueAux (map Prod.fst xs) acc).length
+  = (uniqueAux (map Prod.fst (findMatches xs k).snd) acc).length :=
+by induction xs with
+   | nil => intros; simp [uniqueAux]
+   | cons x xs ih =>
+     intros acc hk
+     simp only [length, uniqueAux]
+     cases Decidable.em (x.fst ∈ acc) with
+     | inl hin =>
+       simp only [hin, ite_true, findMatches]
+       rw [ih _ hk]
+       cases Decidable.em (x.1 = k) with
+       | inl heq => simp only [heq, ite_true]
+       | inr hneq => simp only [hneq, ite_false, map, uniqueAux, hin, ite_true]
+     | inr hout =>
+       simp only [hout, ite_false, findMatches]
+       cases Decidable.em (x.1 = k) with
+       | inl heq =>
+         apply absurd hk
+         rw [heq] at hout
+         exact hout
+       | inr hneq =>
+         rw [ih _ (List.Mem.tail _ hk)]
+         simp only [hneq, ite_false, uniqueAux, hout]
+
+theorem List.length_uniqueAux_singleton_acc {α} [DecidableEq α]
+  (xs : List α) (y : α) (h : ¬ (y ∈ xs)) :
+  length (unique xs) + 1 = length (uniqueAux xs [y]) :=
+by cases xs with
+   | nil => simp [unique, uniqueAux]
+   | cons x xs => 
+     have h_flip : ¬ (x ∈ [y]) := by
+       intro hneg
+       cases hneg with
+       | head => apply h $ List.Mem.head _ _
+       | tail _ => contradiction
+     simp only [unique, uniqueAux, List.not_mem_nil, h, ite_false, h_flip]
+     admit
+
+instance (y : Nat) : Decidable (∀ x : Nat, x - y = x) :=
+if h : y = 0
+then Decidable.isTrue (λ x => by rw [h]; simp)
+else Decidable.isFalse (λ x => by
+  have h1 : 1 - y = 1 := x 1
+  have : y > 0 := Nat.zero_lt_of_ne_zero h
+  have := Nat.sub_lt (Nat.lt.base 0) this
+  apply absurd h1
+  apply Nat.ne_of_lt this
+)
+
+theorem List.length_unique'_findMatches {κ ν} [DecidableEq κ] (xs : List (κ × ν)) (k : κ) :
+  unique' (map Prod.fst xs)
+  = unique' (map Prod.fst (findMatches xs k).snd) := by
+  induction xs with
+  | nil => rfl
+  | cons x xs ih =>
+    simp only [length, unique']
+    rw [ih]
+    cases Decidable.em (∀ (y : κ), y ∈ unique' (map Prod.fst (findMatches xs k).snd) → x.fst ≠ y) with
+    | inl hnew =>
+      rw [if_pos hnew]
+      simp only [findMatches]
+      cases Decidable.em (x.1 = k) with
+      | inl heq =>
+        simp only [heq, ite_true]
+        
+      | inr hneq =>
+        simp only [hneq, ite_false, map, unique']
+        rw [if_pos hnew]
+    | inr hseen =>
+      rw [if_neg hseen]
+      simp only [findMatches]
+      cases Decidable.em (x.1 = k) with
+      | inl heq => simp only [heq, ite_true]
+      | inr hneq =>
+        simp only [hneq, ite_false, map, unique']
+        rw [if_neg hseen]
+
+    -- cases Decidable.em (∀ (y : κ), y ∈ unique' (map Prod.fst xs) → x.fst ≠ y) with
+    -- | inl hnew =>
+    --   rw [if_pos hnew]
+    --   simp only [findMatches]
+    --   cases (Decidable.em (x.1 = k)) with
+    --   | inl heq =>
+    --     rw [ih] at hnew
+    --     apply absurd heq
+    --     apply hnew
+    --   | inr hneq =>
+    --     simp only [hneq, ite_false, map, unique']
+    --     rw [if_pos, ih]
+    --     . intros y hy
+    --       rw [←ih] at hy
+    --       apply hnew _ hy
+    -- | inr hseen =>
+    --   rw [if_neg hseen]
+    --   simp only [findMatches]
+    --   cases Decidable.em (x.1 = k) with
+    --   | inl heq => simp only [heq, ite_true, ih]
+    --   | inr hneq =>
+    --     simp only [hneq, ite_false, map, unique']
+    --     conv => rhs; rw [←ih, if_neg hseen]
+
+
+    -- simp only [length, unique']
+    -- cases Decidable.em (∀ (y : κ), y ∈ unique' (map Prod.fst xs) → x.fst ≠ y) with
+    -- | inl hnew =>
+    --   rw [if_pos hnew]
+    --   simp only [length]
+    --   simp only [findMatches]
+    --   cases Decidable.em (x.1 = k) with
+    --   | inl heq => admit
+    --   | inr hneq =>
+    --     simp only [hneq, ite_false, map, length, unique']
+    --     rw [ih, if_pos]
+    --     . simp
+    --     . intros y hy
+
+
+
+theorem List.length_groupByKey' {κ} [DecidableEq κ] {ν} :
+  ∀ (xs : List (κ × ν)),
+  length (groupByKey xs) = (xs.map Prod.fst).unique'.length
+| [] => rfl
+| (k, v) :: xs => by
+  have ih := length_groupByKey' (findMatches xs k).2
+  simp only [map, unique', groupByKey]
+  simp only [length]
+  rw [ih]
+  -- Recall `findMatches_snd_keys_neq_k`!
+  have htmp : (∀ (y : κ), y ∈ unique' (map Prod.fst (findMatches xs k).2) → (k ≠ y)) := sorry
+  rw [if_pos]
+  simp only [length]
+  apply congrArg (·+1)
+  rw [←length_unique'_findMatches _ k]
+  exact htmp
+
+theorem List.length_groupByKey {κ} [DecidableEq κ] {ν} :
+  ∀ (xs : List (κ × ν)),
+  length (groupByKey xs) = (xs.map Prod.fst).unique.length
+| [] => rfl
+| (k, v) :: xs => by
+  have hterm : length (findMatches xs k).snd < Nat.succ (length xs) :=
+    Nat.lt_of_succ_le $ Nat.succ_le_succ $ findMatches_snd_length xs k
+  have ih := length_groupByKey (findMatches xs k).2
+  simp only [map, unique, uniqueAux, List.not_mem_nil, ite_false, groupByKey]
+  simp only [length]
+  rw [length_uniqueAux_findMatches _ k _ $ List.Mem.head _ _]
+  rw [ih]
+  have := findMatches_snd_keys_neq_k (k := k) xs
+  apply Eq.symm
+  apply List.length_uniqueAux (acc := [k])
+  intro x
+  rw [mem_singleton_iff]
+  apply findMatches_snd_keys_neq_k_map (k := k) xs
+termination_by length_groupByKey xs => length xs
+decreasing_by assumption
+  -- simp only [unique]
+  -- rw [←length_uniqueAux_findMatches (acc := [k]) _ _ $ List.Mem.head _ _]
+  -- have : length (uniqueAux (map Prod.fst xs) [k]) = length (unique (map Prod.fst ((k, v) :: xs))) := rfl
+  -- rw [this]
+  
+
+-- :=
+-- by intros xs
+--    induction xs with
+--    | nil => rfl
+--    | cons x xs ih =>
+--      cases x with | mk k v =>
+--      simp only [map, unique, uniqueAux, List.not_mem_nil, ite_false, groupByKey]
+--      have h_len_succ :
+--       length ((k, v :: (findMatches xs k).fst)
+--               :: groupByKey (findMatches xs k).snd)
+--       = 1 + length (groupByKey (findMatches xs k).2) :=
+--         by simp only [length, Nat.add_comm]
+--      rw [h_len_succ]
+--      rw [length_uniqueAux_findMatches _ k _ $ List.Mem.head k []]
+     -- This won't be structural b/c the inductive call is going to be one
+     -- (findMatches xs k).2
+     -- ^ actually, I'm not sure, because the RHS is still in terms of xs...
+    
+
 -- TODO: as with `count`, should we enforce some sort of constraint on κ to
 -- allow for optimizations (e.g, RBTs)?
 -- FIXME: we need to allow for schema' to have a different η, but this leads
@@ -444,23 +1050,9 @@ def groupBy {η'} [DecidableEq η']
             (project : Row schema → ν)
             (aggregate : κ → List ν → Row schema')
     : Table schema' :=
-  let rec group : List (κ × ν) → List (κ × List ν) := λ
-    | [] => []
-    | (k, v) :: kvs =>
-      let fms := findMatches kvs k
-      have h_help : List.length (findMatches kvs k).snd
-                      < Nat.succ (List.length kvs) :=
-        by apply Nat.lt_of_succ_le
-           apply Nat.succ_le_succ
-           apply findMatches_snd_length
-      (k, v :: fms.1) :: group fms.2
   let projected := t.rows.map (λ r => (key r, project r))
-  let grouped := group projected
+  let grouped := projected.groupByKey
 {rows := grouped.map (λ klv => aggregate klv.1 klv.2)}
-termination_by group xs => xs.length
--- Use this because the default tactic (whatever it is) keeps needlessly
--- introducing dependence on `Quot.sound`
-decreasing_by assumption
 
 /--
 `flattenOne` takes a list of row copies and clean-row templates (i.e., a list of
